<!DOCTYPE rdf:RDF [
    <!ENTITY rdf "http://www.w3.org/1999/02/22-rdf-syntax-ns#" >
    <!ENTITY owl "http://www.w3.org/2002/07/owl#" >
    <!ENTITY xsd "http://www.w3.org/2001/XMLSchema#" >
    <!ENTITY rdfs "http://www.w3.org/2000/01/rdf-schema#" >
    <!ENTITY dc "http://purl.org/dc/elements/1.1/" >
    <!ENTITY wfact "http://williamrobertfunk.com/ontologies/world-factbook#" >
    <!ENTITY pos "http://www.w3.org/2003/01/geo/wgs84_pos#">
    <!ENTITY asset "http://www.daedafusion.com/Asset#">
    <!ENTITY dbpCountry "http://dbpedia.org/ontology/Country#">
]>

<rdf:RDF xmlns="http://www.w3.org/2002/07/owl#"
  xmlns:rdf="http://www.w3.org/1999/02/22-rdf-syntax-ns#"
  xmlns:owl="http://www.w3.org/2002/07/owl#"
  xmlns:xsd="http://www.w3.org/2001/XMLSchema#"
  xmlns:rdfs="http://www.w3.org/2000/01/rdf-schema#"
  xmlns:dc="http://purl.org/dc/elements/1.1/"
  xmlns:wfact="http://williamrobertfunk.com/ontologies/world-factbook#"
  xmlns:pos="http://www.w3.org/2003/01/geo/wgs84_pos#"
  xmlns:asset="http://www.daedafusion.com/Asset#"
  xmlns:dbpCountry="http://dbpedia.org/ontology/Country#"
>

  <Ontology rdf:about="http://williamrobertfunk.com/ontologies/world-factbook">
    <versionInfo rdf:datatype="&xsd;decimal">1.0.2</versionInfo>
    <dc:rights>Copyright 2019 William R.A.D. Funk. All rights reserved.</dc:rights>
    <dc:creator>William R.A.D. Funk</dc:creator>
    <dc:contributor>William R.A.D. Funk</dc:contributor>
    <rdfs:comment>
      Identifies application specific classes and annotations that are relevant
      only to my associated applications.
    </rdfs:comment>
    <rdfs:label>Funk Ontology</rdfs:label>
  </Ontology>

  <!--
  ///////////////////////////////////////////////////////////////////////////////////////
  //
  // Classes
  //
  ///////////////////////////////////////////////////////////////////////////////////////
  -->

  <!-- http://williamrobertfunk.com/ontologies/world-factbook#Country -->

  <rdfs:Class rdf:about="&wfact;Country">
    <rdfs:label>Country</rdfs:label>
    <rdfs:comment>a nation with its own government, occupying a particular territory.</rdfs:comment>
    <owl:equivalentClass rdf:resource="&dbpCountry;" />
  </rdfs:Class>

  <!-- http://williamrobertfunk.com/ontologies/world-factbook#NationalFlag -->

  <rdfs:Class rdf:about="&wfact;NationalFlag">
    <rdfs:label>NationalFlag</rdfs:label>
    <rdfs:comment>
      a piece of cloth flown by the government of a country,
      and designed with specific meanings for its colours and symbols.
    </rdfs:comment>
  </rdfs:Class>

  <!-- http://williamrobertfunk.com/ontologies/world-factbook#Image -->

  <rdfs:Class rdf:about="&wfact;Image">
    <rdfs:subClassOf rdf:resource="&asset;Asset"/>
    <rdfs:label>Image</rdfs:label>
    <rdfs:comment>a digitally stored image</rdfs:comment>
  </rdfs:Class>

  <!-- http://williamrobertfunk.com/ontologies/world-factbook#BorderMap -->

  <rdfs:Class rdf:about="&wfact;BorderMap">
    <rdfs:subClassOf rdf:resource="&wfact;Image"/>
    <rdfs:label>Border Map Image</rdfs:label>
    <rdfs:comment>an image showing a country's full border and direct neighbors.</rdfs:comment>
  </rdfs:Class>

  <!-- http://williamrobertfunk.com/ontologies/world-factbook#RegionMap -->

  <rdfs:Class rdf:about="&wfact;RegionMap">
    <rdfs:subClassOf rdf:resource="&wfact;Image"/>
    <rdfs:label>Region Map Image</rdfs:label>
    <rdfs:comment>an image showing a country's position within a region.</rdfs:comment>
  </rdfs:Class>

  <!-- http://williamrobertfunk.com/ontologies/world-factbook#DomainArea -->

  <rdfs:Class rdf:about="&wfact;DomainArea">
    <rdfs:label>Domain Area</rdfs:label>
    <rdfs:comment>Area within a country's borders (ie. Land, Water, Total).</rdfs:comment>
  </rdfs:Class>

  <!-- http://williamrobertfunk.com/ontologies/world-factbook#Coast -->

  <rdfs:Class rdf:about="&wfact;Coast">
    <rdfs:label>Coast</rdfs:label>
    <rdfs:comment>Geographic section where the land borders the sea.</rdfs:comment>
  </rdfs:Class>

  <!-- http://williamrobertfunk.com/ontologies/world-factbook#Climate -->

  <rdfs:Class rdf:about="&wfact;Climate">
    <rdfs:label>Climate</rdfs:label>
    <rdfs:comment>The weather conditions prevailing in an area in general or over a long period.</rdfs:comment>
  </rdfs:Class>

  <!-- http://williamrobertfunk.com/ontologies/world-factbook#ClimateZone -->

  <rdfs:Class rdf:about="&wfact;ClimateZone">
    <rdfs:label>Climate Zone</rdfs:label>
    <rdfs:comment>
      Divisions of the Earth's climates into general climate zones according to average temperatures and average rainfall.
      The three major climate zones on the Earth are the polar, temperate, and tropical zones.
    </rdfs:comment>
  </rdfs:Class>

  <!-- http://williamrobertfunk.com/ontologies/world-factbook#BorderCountryPair -->

  <rdfs:Class rdf:about="&wfact;BorderCountryPair">
    <rdfs:label>Border Country Pair</rdfs:label>
    <rdfs:comment>Two countries that share a land border.</rdfs:comment>
  </rdfs:Class>

  <!-- http://williamrobertfunk.com/ontologies/world-factbook#Border -->

  <rdfs:Class rdf:about="&wfact;Border">
    <rdfs:label>National Border</rdfs:label>
    <rdfs:comment>Total border belonging to a soverign nation.</rdfs:comment>
  </rdfs:Class>

  <!-- http://williamrobertfunk.com/ontologies/world-factbook#MaritimeClaim -->

  <rdfs:Class rdf:about="&wfact;MaritimeClaim">
    <rdfs:label>Maritime Claim</rdfs:label>
    <rdfs:comment>
      The adjacent belt of sea that extends beyond a coastal state's land territory and internal waters.
      Includes airspace over that belt of sea.
    </rdfs:comment>
  </rdfs:Class>

  <!-- http://williamrobertfunk.com/ontologies/world-factbook#NaturalResource -->

  <rdfs:Class rdf:about="&wfact;NaturalResource">
    <rdfs:label>Natural Resource</rdfs:label>
    <rdfs:comment>
      Material or substance such as minerals, forests, water,and fertile land
      that occur in nature and can be used for economic gain.
    </rdfs:comment>
  </rdfs:Class>

  <!-- http://williamrobertfunk.com/ontologies/world-factbook#Terrain -->

  <rdfs:Class rdf:about="&wfact;Terrain">
    <rdfs:label>Natural Resource</rdfs:label>
    <rdfs:comment>A stretch of land, especially with regard to its physical features.</rdfs:comment>
  </rdfs:Class>

  <!--
  ///////////////////////////////////////////////////////////////////////////////////////
  //
  // Object Properties
  //
  ///////////////////////////////////////////////////////////////////////////////////////
  -->

  <!-- http://williamrobertfunk.com/ontologies/world-factbook#hasNationalFlag -->

  <owl:ObjectProperty rdf:about="&wfact;hasNationalFlag">
      <rdfs:domain rdf:resource="&wfact;Country"/>
      <rdfs:range rdf:resource="&wfact;NationalFlag"/>
  </owl:ObjectProperty>

  <!-- http://williamrobertfunk.com/ontologies/world-factbook#hasBorderMap -->

  <owl:ObjectProperty rdf:about="&wfact;hasBorderMap">
      <rdfs:domain rdf:resource="&wfact;Country"/>
      <rdfs:range rdf:resource="&wfact;BorderMap"/>
  </owl:ObjectProperty>

  <!-- http://williamrobertfunk.com/ontologies/world-factbook#hasRegionMap -->

  <owl:ObjectProperty rdf:about="&wfact;hasRegionMap">
      <rdfs:domain rdf:resource="&wfact;Country"/>
      <rdfs:range rdf:resource="&wfact;RegionMap"/>
  </owl:ObjectProperty>

  <!-- http://williamrobertfunk.com/ontologies/world-factbook#hasSupplementalImage -->

  <owl:ObjectProperty rdf:about="&wfact;hasSupplementalImage">
      <rdfs:domain rdf:resource="&wfact;Country"/>
      <rdfs:range rdf:resource="&wfact;Image"/>
  </owl:ObjectProperty>

  <!-- http://williamrobertfunk.com/ontologies/world-factbook#hasDomainArea -->

  <owl:ObjectProperty rdf:about="&wfact;hasSupplementalImage">
      <rdfs:domain rdf:resource="&wfact;Country"/>
      <rdfs:range rdf:resource="&wfact;DomainArea"/>
  </owl:ObjectProperty>

  <!-- http://williamrobertfunk.com/ontologies/world-factbook#hasCoast -->

  <owl:ObjectProperty rdf:about="&wfact;hasCoast">
      <rdfs:domain rdf:resource="&wfact;Country"/>
      <rdfs:range rdf:resource="&wfact;Coast"/>
  </owl:ObjectProperty>

  <!-- http://williamrobertfunk.com/ontologies/world-factbook#hasClimate -->

  <owl:ObjectProperty rdf:about="&wfact;hasClimate">
      <rdfs:domain rdf:resource="&wfact;Country"/>
      <rdfs:range rdf:resource="&wfact;Climate"/>
  </owl:ObjectProperty>

  <!-- http://williamrobertfunk.com/ontologies/world-factbook#hasClimateZone -->

  <owl:ObjectProperty rdf:about="&wfact;hasClimateZone">
      <rdfs:domain rdf:resource="&wfact;Climate"/>
      <rdfs:range rdf:resource="&wfact;ClimateZone"/>
  </owl:ObjectProperty>

  <!-- http://williamrobertfunk.com/ontologies/world-factbook#hasBorderCountryPair -->

  <owl:ObjectProperty rdf:about="&wfact;hasBorderCountryPair">
      <rdfs:domain rdf:resource="&wfact;Country"/>
      <rdfs:range rdf:resource="&wfact;BorderCountryPair"/>
  </owl:ObjectProperty>

  <!-- http://williamrobertfunk.com/ontologies/world-factbook#hasCountry -->

  <owl:ObjectProperty rdf:about="&wfact;hasCountry">
      <rdfs:domain rdf:resource="&wfact;BorderCountryPair"/>
      <rdfs:range rdf:resource="&wfact;Country"/>
  </owl:ObjectProperty>

  <!-- http://williamrobertfunk.com/ontologies/world-factbook#hasBorder -->

  <owl:ObjectProperty rdf:about="&wfact;hasBorder">
      <rdfs:domain rdf:resource="&wfact;Country"/>
      <rdfs:range rdf:resource="&wfact;Border"/>
  </owl:ObjectProperty>

  <!-- http://williamrobertfunk.com/ontologies/world-factbook#hasMaritimeClaim -->

  <owl:ObjectProperty rdf:about="&wfact;hasMaritimeClaim">
      <rdfs:domain rdf:resource="&wfact;Country"/>
      <rdfs:range rdf:resource="&wfact;MaritimeClaim"/>
  </owl:ObjectProperty>

  <!-- http://williamrobertfunk.com/ontologies/world-factbook#hasNaturalResource -->

  <owl:ObjectProperty rdf:about="&wfact;hasNaturalResource">
      <rdfs:domain rdf:resource="&wfact;Country"/>
      <rdfs:range rdf:resource="&wfact;NaturalResource"/>
  </owl:ObjectProperty>

  <!-- http://williamrobertfunk.com/ontologies/world-factbook#hasTerrain -->

  <owl:ObjectProperty rdf:about="&wfact;hasTerrain">
      <rdfs:domain rdf:resource="&wfact;Country"/>
      <rdfs:range rdf:resource="&wfact;Terrain"/>
  </owl:ObjectProperty>

  <!--
  ///////////////////////////////////////////////////////////////////////////////////////
  //
  // Datatype Properties
  //
  ///////////////////////////////////////////////////////////////////////////////////////
  -->

  <!-- http://williamrobertfunk.com/ontologies/world-factbook#background -->

  <DatatypeProperty rdf:about="&wfact;background">
    <rdfs:label>Background information</rdfs:label>
    <rdfs:comment>Description of variable length that summarizes the history of a thing.</rdfs:comment>
    <rdf:type rdf:resource="&owl;FunctionalProperty" />
    <rdfs:domain rdf:resource="&wfact;Country"/>
    <rdfs:range rdf:resource="&xsd;string"/>
  </DatatypeProperty>

  <!-- http://williamrobertfunk.com/ontologies/world-factbook#imageDimensions -->

  <DatatypeProperty rdf:about="&wfact;imageDimensions">
    <rdfs:label>Width by Height Dimensions</rdfs:label>
    <rdfs:comment>The width and height of the image, usually in pixels</rdfs:comment>
    <rdf:type rdf:resource="&owl;FunctionalProperty" />
    <rdfs:domain rdf:resource="&wfact;Image"/>
    <rdfs:range rdf:resource="&xsd;string"/>
  </DatatypeProperty>

  <!-- http://williamrobertfunk.com/ontologies/world-factbook#imageSize -->

  <DatatypeProperty rdf:about="&wfact;imageSize">
    <rdfs:label>Image Size</rdfs:label>
    <rdfs:comment>The amount of computer memory the image requires.</rdfs:comment>
    <rdf:type rdf:resource="&owl;FunctionalProperty" />
    <rdfs:domain rdf:resource="&wfact;Image"/>
    <rdfs:range rdf:resource="&xsd;string"/>
  </DatatypeProperty>

  <!-- http://williamrobertfunk.com/ontologies/world-factbook#locationDescription -->

  <DatatypeProperty rdf:about="&wfact;locationDescription">
    <rdfs:label>Location Description</rdfs:label>
    <rdfs:comment>A description of where in the world the country is located.</rdfs:comment>
    <rdfs:domain rdf:resource="&wfact;Country"/>
    <rdfs:range rdf:resource="&xsd;string"/>
  </DatatypeProperty>

  <!-- http://williamrobertfunk.com/ontologies/world-factbook#mapReferences -->

  <DatatypeProperty rdf:about="&wfact;mapReferences">
    <rdfs:label>Map Reference</rdfs:label>
    <rdfs:comment>A broad reference to country's position in the world (ie. Africa).</rdfs:comment>
    <rdfs:domain rdf:resource="&wfact;Country"/>
    <rdfs:range rdf:resource="&xsd;string"/>
  </DatatypeProperty>

  <!-- http://williamrobertfunk.com/ontologies/world-factbook#locatorURI -->

  <DatatypeProperty rdf:about="&wfact;locatorURI">
    <rdfs:label>Locator URL</rdfs:label>
    <rdfs:comment>URL location where image was originally located.</rdfs:comment>
    <rdfs:domain rdf:resource="&asset;Asset"/>
    <rdfs:range rdf:resource="&xsd;literal"/>
  </DatatypeProperty>

  <!-- http://williamrobertfunk.com/ontologies/world-factbook#contentDescription -->

  <DatatypeProperty rdf:about="&wfact;contentDescription">
    <rdfs:label>Content Description</rdfs:label>
    <rdfs:comment>Description of the contents contained within the asset.</rdfs:comment>
    <rdfs:domain rdf:resource="&asset;Asset"/>
    <rdfs:range rdf:resource="&xsd;string"/>
  </DatatypeProperty>

  <!-- http://williamrobertfunk.com/ontologies/world-factbook#unit -->

  <DatatypeProperty rdf:about="&wfact;unit">
    <rdfs:label>Unit</rdfs:label>
    <rdfs:comment>Unit of measurement (ie. km, mi, sq km, celcius, etc.).</rdfs:comment>
    <rdfs:domain rdf:resource="&asset;DomainArea"/>
    <rdfs:domain rdf:resource="&asset;Coast"/>
    <rdfs:domain rdf:resource="&asset;BorderCountryPair"/>
    <rdfs:domain rdf:resource="&asset;Border"/>
    <rdfs:domain rdf:resource="&asset;MaritimeClaim"/>
    <rdfs:range rdf:resource="&xsd;string"/>
  </DatatypeProperty>

  <!-- http://williamrobertfunk.com/ontologies/world-factbook#totalArea -->

  <DatatypeProperty rdf:about="&wfact;totalArea">
    <rdfs:label>Total Area</rdfs:label>
    <rdfs:comment>Total area associated with the entity to which it's attached.</rdfs:comment>
    <rdfs:domain rdf:resource="&asset;DomainArea"/>
    <rdfs:range rdf:resource="&xsd;string"/>
  </DatatypeProperty>

  <!-- http://williamrobertfunk.com/ontologies/world-factbook#landArea -->

  <DatatypeProperty rdf:about="&wfact;landArea">
    <rdfs:label>Land Area</rdfs:label>
    <rdfs:comment>Total land area associated with the entity to which it's attached.</rdfs:comment>
    <rdfs:domain rdf:resource="&asset;DomainArea"/>
    <rdfs:range rdf:resource="&xsd;string"/>
  </DatatypeProperty>

  <!-- http://williamrobertfunk.com/ontologies/world-factbook#waterArea -->

  <DatatypeProperty rdf:about="&wfact;waterArea">
    <rdfs:label>Water Area</rdfs:label>
    <rdfs:comment>Total water area associated with the entity to which it's attached.</rdfs:comment>
    <rdfs:domain rdf:resource="&asset;DomainArea"/>
    <rdfs:range rdf:resource="&xsd;string"/>
  </DatatypeProperty>

  <!-- http://williamrobertfunk.com/ontologies/world-factbook#areaRank -->

  <DatatypeProperty rdf:about="&wfact;areaRank">
    <rdfs:label>Area Rank</rdfs:label>
    <rdfs:comment>Numerical rank compared to similar entities.</rdfs:comment>
    <rdfs:domain rdf:resource="&asset;DomainArea"/>
    <rdfs:range rdf:resource="&xsd;integer"/>
  </DatatypeProperty>

  <!-- http://williamrobertfunk.com/ontologies/world-factbook#areaComparative -->

  <DatatypeProperty rdf:about="&wfact;areaComparative">
    <rdfs:label>Comparative Area</rdfs:label>
    <rdfs:comment>Comparative association with a well-known area to better define scale qualitatively.</rdfs:comment>
    <rdfs:domain rdf:resource="&asset;DomainArea"/>
    <rdfs:range rdf:resource="&xsd;string"/>
  </DatatypeProperty>

  <!-- http://williamrobertfunk.com/ontologies/world-factbook#length -->

  <DatatypeProperty rdf:about="&wfact;length">
    <rdfs:label>Length</rdfs:label>
    <rdfs:comment>The measurement or extent of something from end to end</rdfs:comment>
    <rdfs:domain rdf:resource="&asset;Coast"/>
    <rdfs:range rdf:resource="&xsd;string"/>
  </DatatypeProperty>

  <!-- http://williamrobertfunk.com/ontologies/world-factbook#lengthModifier -->

  <DatatypeProperty rdf:about="&wfact;lengthModifier">
    <rdfs:label>Length Modifier</rdfs:label>
    <rdfs:comment>An additional descriptor to add information to a simple length measurement.</rdfs:comment>
    <rdfs:domain rdf:resource="&asset;Coast"/>
    <rdfs:range rdf:resource="&xsd;string"/>
  </DatatypeProperty>

  <!-- http://williamrobertfunk.com/ontologies/world-factbook#climateZoneName -->

  <DatatypeProperty rdf:about="&wfact;climateZoneName">
    <rdfs:label>Climate Zone Name</rdfs:label>
    <rdfs:comment>Name of the climate zone (ie. polar, temperate, etc.).</rdfs:comment>
    <rdfs:domain rdf:resource="&asset;ClimateZone"/>
    <rdfs:range rdf:resource="&xsd;string"/>
  </DatatypeProperty>

  <!-- http://williamrobertfunk.com/ontologies/world-factbook#climateZoneDescription -->

  <DatatypeProperty rdf:about="&wfact;climateZoneDescription">
    <rdfs:label>Climate Zone Description</rdfs:label>
    <rdfs:comment>Greater detail for the climate of a given area.</rdfs:comment>
    <rdfs:domain rdf:resource="&asset;ClimateZone"/>
    <rdfs:range rdf:resource="&xsd;string"/>
  </DatatypeProperty>

  <!-- http://williamrobertfunk.com/ontologies/world-factbook#borderLength -->

  <DatatypeProperty rdf:about="&wfact;borderLength">
    <rdfs:label>Border Length</rdfs:label>
    <rdfs:comment>Length of distance by land that one country shares with other countries.</rdfs:comment>
    <rdfs:domain rdf:resource="&asset;BorderCountryPair"/>
    <rdfs:range rdf:resource="&xsd;string"/>
  </DatatypeProperty>

  <!-- http://williamrobertfunk.com/ontologies/world-factbook#totalLandBorder -->

  <DatatypeProperty rdf:about="&wfact;totalLandBorder">
    <rdfs:label>Total Land Border</rdfs:label>
    <rdfs:comment>Total length of distance by land of a country's border.</rdfs:comment>
    <rdfs:domain rdf:resource="&asset;Border"/>
    <rdfs:range rdf:resource="&xsd;string"/>
  </DatatypeProperty>

  <!-- http://williamrobertfunk.com/ontologies/world-factbook#totalBorderCountries -->

  <DatatypeProperty rdf:about="&wfact;totalBorderCountries">
    <rdfs:label>Total Border Countries</rdfs:label>
    <rdfs:comment>Total number of countries sharing a border with this nation.</rdfs:comment>
    <rdfs:domain rdf:resource="&asset;Border"/>
    <rdfs:range rdf:resource="&xsd;integer"/>
  </DatatypeProperty>

  <!-- http://williamrobertfunk.com/ontologies/world-factbook#territorialSea -->

  <DatatypeProperty rdf:about="&wfact;territorialSea">
    <rdfs:label>Territorial Sea</rdfs:label>
    <rdfs:comment>Length of sea belt belonging to sovereign coastal state.</rdfs:comment>
    <rdfs:domain rdf:resource="&asset;MaritimeClaim"/>
    <rdfs:range rdf:resource="&xsd;integer"/>
  </DatatypeProperty>

  <!-- http://williamrobertfunk.com/ontologies/world-factbook#exclusiveEconomicZone -->

  <DatatypeProperty rdf:about="&wfact;exclusiveEconomicZone">
    <rdfs:label>Territorial Sea</rdfs:label>
    <rdfs:comment>Length of sea belt belonging to sovereign coastal state for exclusive economic use.</rdfs:comment>
    <rdfs:domain rdf:resource="&asset;MaritimeClaim"/>
    <rdfs:range rdf:resource="&xsd;integer"/>
  </DatatypeProperty>

  <!-- http://williamrobertfunk.com/ontologies/world-factbook#contiguousZone -->

  <DatatypeProperty rdf:about="&wfact;contiguousZone">
    <rdfs:label>Contiguous Zone</rdfs:label>
    <rdfs:comment>
      Length of sea belt belonging to sovereign coastal state for legally protecting against infringement of its customs,
      fiscal, immigration, or sanitary laws and regulations.
    </rdfs:comment>
    <rdfs:domain rdf:resource="&asset;MaritimeClaim"/>
    <rdfs:range rdf:resource="&xsd;integer"/>
  </DatatypeProperty>

  <!-- http://williamrobertfunk.com/ontologies/world-factbook#continentalShelf -->

  <DatatypeProperty rdf:about="&wfact;continentalShelf">
    <rdfs:label>Continental Shelf</rdfs:label>
    <rdfs:comment>
      Length of sea belt belonging to sovereign coastal state with exclusive jurisdiction for the purpose of exploring it
      and exploiting its natural resources.
    </rdfs:comment>
    <rdfs:domain rdf:resource="&asset;MaritimeClaim"/>
    <rdfs:range rdf:resource="&xsd;integer"/>
  </DatatypeProperty>

  <!-- http://williamrobertfunk.com/ontologies/world-factbook#continentalShelfModifier -->

  <DatatypeProperty rdf:about="&wfact;continentalShelfModifier">
    <rdfs:label>Continental Shelf</rdfs:label>
    <rdfs:comment>
      Additions, subtractions, or exceptions that pertain to the length of sea belt belonging to a soverign coastal state.
    </rdfs:comment>
    <rdfs:domain rdf:resource="&asset;MaritimeClaim"/>
    <rdfs:range rdf:resource="&xsd;string"/>
  </DatatypeProperty>

  <!-- http://williamrobertfunk.com/ontologies/world-factbook#supplementalExplanation -->

  <DatatypeProperty rdf:about="&wfact;supplementalExplanation">
    <rdfs:label>supplementalExplanation</rdfs:label>
    <rdfs:comment>
      When details are given that don't readily fit into any given category, they go here.
    </rdfs:comment>
    <rdfs:domain rdf:resource="&asset;MaritimeClaim"/>
    <rdfs:range rdf:resource="&xsd;string"/>
  </DatatypeProperty>

  <!-- http://williamrobertfunk.com/ontologies/world-factbook#exclusiveFishingZone -->

  <DatatypeProperty rdf:about="&wfact;exclusiveFishingZone">
    <rdfs:label>exclusiveFishingZone</rdfs:label>
    <rdfs:comment>
      An area beyond the outer limit of the territorial sea in which the coastal State has the right to fish,
      subject to any concessions which may be granted to foreign fishermen.
    </rdfs:comment>
    <rdfs:domain rdf:resource="&asset;MaritimeClaim"/>
    <rdfs:range rdf:resource="&xsd;string"/>
  </DatatypeProperty>

  <!-- http://williamrobertfunk.com/ontologies/world-factbook#resourceName -->

  <DatatypeProperty rdf:about="&wfact;resourceName">
    <rdfs:label>resourceName</rdfs:label>
    <rdfs:comment>The name of the resource (ie. coal, copper, salt, fish)</rdfs:comment>
    <rdfs:domain rdf:resource="&asset;NaturalResource"/>
    <rdfs:range rdf:resource="&xsd;string"/>
  </DatatypeProperty>

  <!-- http://williamrobertfunk.com/ontologies/world-factbook#description -->

  <DatatypeProperty rdf:about="&wfact;description">
    <rdfs:label>description</rdfs:label>
    <rdfs:comment>Description of the terrain</rdfs:comment>
    <rdfs:domain rdf:resource="&asset;NaturalResource"/>
    <rdfs:range rdf:resource="&xsd;string"/>
  </DatatypeProperty>

</rdf:RDF>