{
  "@context": {
    "aircraft": "http://williamrobertfunk.com/ontologies/aircraft#",
    "blade": "http://modusoperandi.com/ont/blade#",
    "dbp": "http://dbpedia.org/ontology",
    "dc": "http://purl.org/dc/elements/1.1/",
    "foaf": "http://xmlns.com/foaf/0.1/",
    "general": "http://williamrobertfunk.com/ontologies/general#",
    "owl": "http://www.w3.org/2002/07/owl#",
    "pos": "http://www.w3.org/2003/01/geo/wgs84_pos#",
    "rdf": "http://www.w3.org/1999/02/22-rdf-syntax-ns#",
    "rdfs": "http://www.w3.org/2000/01/rdf-schema#",
    "xsd": "http://www.w3.org/2001/XMLSchema#"
  },
  "@graph": [
    {
      "@id": "aircraft:numberOfLandingPointSize1",
      "@type": "owl:DatatypeProperty",
      "rdfs:comment": "\n      Number of places in a Helicopter Landing Zone that contain three unobstructed concentric circles of\n      5, 15, and 25 meters in diameter respectively from inside out.\n\n      Light observation helicopters such as the OH-6 and OH-58D.\n    ",
      "rdfs:domain": {
        "@id": "aircraft:HelicopterLandingZone"
      },
      "rdfs:range": {
        "@id": "xsd:integer"
      }
    },
    {
      "@id": "aircraft:numberOfLandingPointSize2",
      "@type": "owl:DatatypeProperty",
      "rdfs:comment": "\n      Number of places in a Helicopter Landing Zone that contain three unobstructed concentric circles of\n      10, 20, and 35 meters in diameter respectively from inside out.\n\n      Light utility and attack helicopters such as the UH-1H, H-65, and AH-1W.\n    ",
      "rdfs:domain": {
        "@id": "aircraft:HelicopterLandingZone"
      },
      "rdfs:range": {
        "@id": "xsd:integer"
      }
    },
    {
      "@id": "aircraft:numberOfLandingPointSize3",
      "@type": "owl:DatatypeProperty",
      "rdfs:comment": "\n      Number of places in a Helicopter Landing Zone that contain three unobstructed concentric circles of\n      15, 35, and 50 meters in diameter respectively from inside out.\n\n      Medium utility and attack helicopters such as the UH-60, H-2, and AH-64.\n    ",
      "rdfs:domain": {
        "@id": "aircraft:HelicopterLandingZone"
      },
      "rdfs:range": {
        "@id": "xsd:integer"
      }
    },
    {
      "@id": "aircraft:numberOfLandingPointSize4",
      "@type": "owl:DatatypeProperty",
      "rdfs:comment": "\n      Number of places in a Helicopter Landing Zone that contain three unobstructed concentric circles of\n      15, 35, and 80 meters in diameter respectively from inside out.\n\n      Cargo helicopters such as the CH-47, H-3 and CH-53, or with prior coordination.\n    ",
      "rdfs:domain": {
        "@id": "aircraft:HelicopterLandingZone"
      },
      "rdfs:range": {
        "@id": "xsd:integer"
      }
    },
    {
      "@id": "aircraft:numberOfLandingPointSize5",
      "@type": "owl:DatatypeProperty",
      "rdfs:comment": "\n      Number of places in a Helicopter Landing Zone that contain three unobstructed concentric circles of\n      15, 60, and 100 meters in diameter respectively from inside out.\n\n      Slingload helicopters and aircraft of an unknown origin.\n    ",
      "rdfs:domain": {
        "@id": "aircraft:HelicopterLandingZone"
      },
      "rdfs:range": {
        "@id": "xsd:integer"
      }
    },
    {
      "@id": "aircraft:numberOfLandingPointSize6",
      "@type": "owl:DatatypeProperty",
      "rdfs:comment": "\n      Number of places in a Helicopter Landing Zone that contain three unobstructed concentric circles of\n      15, 75, and 125 meters in diameter respectively from inside out.\n\n      Slingload long-line operations.\n    ",
      "rdfs:domain": {
        "@id": "aircraft:HelicopterLandingZone"
      },
      "rdfs:range": {
        "@id": "xsd:integer"
      }
    },
    {
      "@id": "aircraft:numberOfLandingPointSize7",
      "@type": "owl:DatatypeProperty",
      "rdfs:comment": "\n      Number of places in a Helicopter Landing Zone that contain three unobstructed concentric circles of\n      15, 75, and 150 meters in diameter respectively from inside out.\n\n      Slingload operations with night vision goggles (NVG).\n    ",
      "rdfs:domain": {
        "@id": "aircraft:HelicopterLandingZone"
      },
      "rdfs:range": {
        "@id": "xsd:integer"
      }
    },
    {
      "@id": "general:length",
      "@type": "owl:DatatypeProperty",
      "rdfs:domain": {
        "@id": "aircraft:HelicopterLandingZone"
      }
    },
    {
      "@id": "general:unit",
      "@type": "owl:DatatypeProperty",
      "rdfs:domain": {
        "@id": "aircraft:HelicopterLandingZone"
      }
    },
    {
      "@id": "general:hasSurfaceMaterial",
      "@type": "owl:ObjectProperty",
      "rdfs:domain": {
        "@id": "aircraft:HelicopterLandingZone"
      }
    },
    {
      "@id": "aircraft:hasHelicopterLandingZone",
      "@type": "owl:ObjectProperty",
      "rdfs:range": {
        "@id": "aircraft:HelicopterLandingZone"
      }
    },
    {
      "@id": "aircraft:HelicopterLandingZone",
      "@type": "owl:Class",
      "blade:navClass": true,
      "rdfs:comment": "\n      A specified ground area for landing assault helicopters to embark or disembark troops and/or cargo.\n    ",
      "rdfs:label": "Helicopter Landing Zone"
    },
    {
      "@id": "general:width",
      "@type": "owl:DatatypeProperty",
      "rdfs:domain": {
        "@id": "aircraft:HelicopterLandingZone"
      }
    },
    {
      "@id": "general:hasLocation",
      "@type": "owl:ObjectProperty",
      "rdfs:domain": {
        "@id": "aircraft:HelicopterLandingZone"
      }
    },
    {
      "@id": "http://williamrobertfunk.com/ontologies/aircraft",
      "@type": "owl:Ontology",
      "dc:contributor": "William R.A.D. Funk",
      "dc:creator": "William R.A.D. Funk",
      "dc:rights": "Copyright 2019 William R.A.D. Funk. All rights reserved.",
      "owl:versionInfo": {
        "@type": "xsd:decimal",
        "@value": "1.0"
      },
      "rdfs:comment": "\n      Identifies application specific classes and annotations that are relevant\n      only to my associated applications.\n    ",
      "rdfs:label": "Funk Ontology"
    }
  ]
}