{
    "@context": {
      "airport": "http://williamrobertfunk.com/ontologies/airport#",
      "blade": "http://modusoperandi.com/ont/blade#",
      "dc": "http://purl.org/dc/elements/1.1/",
      "municipality": "http://williamrobertfunk.com/ontologies/municipality#",
      "owl": "http://www.w3.org/2002/07/owl#",
      "rdf": "http://www.w3.org/1999/02/22-rdf-syntax-ns#",
      "rdfs": "http://www.w3.org/2000/01/rdf-schema#",
      "wfact": "http://williamrobertfunk.com/ontologies/world-factbook#",
      "xsd": "http://www.w3.org/2001/XMLSchema#"
    },
    "@graph": [
      {
        "@id": "wfact:hasMunicipality",
        "@type": "owl:ObjectProperty",
        "rdfs:domain": {
          "@id": "municipality:Municipality"
        },
        "rdfs:range": [
          {
            "@id": "wfact:Country"
          },
          {
            "@id": "airport:Airport"
          }
        ]
      },
      {
        "@id": "municipality:Municipality",
        "@type": "owl:Class",
        "blade:navClass": true,
        "rdfs:comment": "\n      a city or town that has corporate status and local government.\n    ",
        "rdfs:label": "Municipality"
      },
      {
        "@id": "airport:name",
        "@type": [
          "owl:DatatypeProperty",
          "owl:FunctionalProperty"
        ],
        "rdfs:comment": "\n      Name or title associated with thing or place it represents.\n    ",
        "rdfs:domain": {
          "@id": "municipality:Municipality"
        },
        "rdfs:label": "Name",
        "rdfs:range": {
          "@id": "xsd:string"
        }
      },
      {
        "@id": "wfact:hasAirport",
        "@type": "owl:ObjectProperty",
        "rdfs:domain": {
          "@id": "municipality:Municipality"
        },
        "rdfs:range": {
          "@id": "airport:Airport"
        }
      },
      {
        "@id": "wfact:hasCountry",
        "@type": "owl:ObjectProperty",
        "rdfs:domain": {
          "@id": "municipality:Municipality"
        },
        "rdfs:range": {
          "@id": "wfact:Country"
        }
      },
      {
        "@id": "http://williamrobertfunk.com/ontologies/municipality",
        "@type": "owl:Ontology",
        "dc:contributor": "William R.A.D. Funk",
        "dc:creator": "William R.A.D. Funk",
        "dc:rights": "Copyright 2019 William R.A.D. Funk. All rights reserved.",
        "owl:versionInfo": {
          "@type": "xsd:decimal",
          "@value": "1.0"
        },
        "rdfs:comment": "\n      Identifies application specific classes and annotations that are relevant\n      only to my associated applications.\n    ",
        "rdfs:label": "Funk Ontology"
      },
      {
        "@id": "wfact:hasLocation",
        "@type": "owl:ObjectProperty",
        "rdfs:domain": {
          "@id": "municipality:Municipality"
        },
        "rdfs:range": {
          "@id": "wfact:Location"
        }
      }
    ]
  }