{
  "@context": {
    "blade": "http://modusoperandi.com/ont/blade#",
    "country": "http://williamrobertfunk.com/ontologies/country#",
    "dc": "http://purl.org/dc/elements/1.1/",
    "foaf": "http://xmlns.com/foaf/0.1/",
    "foaf1": "http://xmlns.com/foaf/0.1",
    "owl": "http://www.w3.org/2002/07/owl#",
    "rdf": "http://www.w3.org/1999/02/22-rdf-syntax-ns#",
    "rdfs": "http://www.w3.org/2000/01/rdf-schema#",
    "wleaders": "http://williamrobertfunk.com/ontologies/world-leaders#",
    "xsd": "http://www.w3.org/2001/XMLSchema#"
  },
  "@graph": [
    {
      "@id": "wleaders:GovernmentOffice",
      "@type": "owl:Class",
      "blade:navClass": true,
      "rdfs:comment": "\n      a title or position in a governing body with a specific set of roles, responsibilities, and authority.\n    ",
      "rdfs:label": "Government Office"
    },
    {
      "@id": "country:hasCountry",
      "@type": "owl:ObjectProperty",
      "rdfs:domain": {
        "@id": "wleaders:GovernmentOffice"
      },
      "rdfs:range": {
        "@id": "country:Country"
      }
    },
    {
      "@id": "wleaders:title",
      "@type": [
        "owl:DatatypeProperty",
        "owl:FunctionalProperty"
      ],
      "rdfs:comment": "\n      The official name of the government office\n    ",
      "rdfs:domain": {
        "@id": "wleaders:GovernmentOffice"
      },
      "rdfs:label": "Title",
      "rdfs:range": {
        "@id": "xsd:string"
      }
    },
    {
      "@id": "wleaders:hasGovernmentOffice",
      "@type": "owl:ObjectProperty",
      "rdfs:domain": {
        "@id": "country:Country"
      },
      "rdfs:range": {
        "@id": "wleaders:GovernmentOffice"
      }
    },
    {
      "@id": "wleaders:hasGovernmentOfficial",
      "@type": "owl:ObjectProperty",
      "rdfs:comment": "\n      a person serving a governing body in the capacity outlined by the government office to which they are employed.\n    ",
      "rdfs:domain": {
        "@id": "wleaders:GovernmentOffice"
      },
      "rdfs:range": {
        "@id": "wleaders:Person"
      }
    },
    {
      "@id": "wleaders:appointedGovernmentOffice",
      "@type": "owl:ObjectProperty",
      "rdfs:comment": "\n      a government office to which this person is appointed.\n    ",
      "rdfs:domain": {
        "@id": "wleaders:Person"
      },
      "rdfs:range": {
        "@id": "wleaders:GovernmentOffice"
      }
    },
    {
      "@id": "wleaders:regionSpecific",
      "@type": [
        "owl:DatatypeProperty",
        "owl:FunctionalProperty"
      ],
      "rdfs:comment": "\n      Specific Region to which the government office applies\n      (ie. \"Chief Executive\" in China for Hong Kong, or Macau).\n    ",
      "rdfs:domain": {
        "@id": "wleaders:GovernmentOffice"
      },
      "rdfs:label": "Region Specific",
      "rdfs:range": {
        "@id": "xsd:string"
      }
    },
    {
      "@id": "http://williamrobertfunk.com/ontologies/world-leaders",
      "@type": "owl:Ontology",
      "dc:contributor": "William R.A.D. Funk",
      "dc:creator": "William R.A.D. Funk",
      "dc:rights": "Copyright 2019 William R.A.D. Funk. All rights reserved.",
      "owl:versionInfo": {
        "@type": "xsd:decimal",
        "@value": "1.1"
      },
      "rdfs:comment": "\n      Identifies application specific classes and annotations that are relevant\n      only to my associated applications.\n    ",
      "rdfs:label": "Funk Ontology"
    },
    {
      "@id": "wleaders:Person",
      "@type": "owl:Class",
      "blade:navClass": true,
      "owl:equivalentClass": {
        "@id": "foaf:Person"
      },
      "rdfs:comment": "\n      a human being regarded as an individual.\n    ",
      "rdfs:label": "Person"
    }
  ]
}